itree unrolling theorems

HOL/testItreeScript.sml
@@ -35,6 +35,178 @@ Proof
   rw[FUN_EQ_THM, Once itree_unfold]
 QED
 
+(* utilities *)
+
+Definition ibind_cb_def[simp]:
+    ibind_cb k (INL (Ret r)) = itree_CASE (k r)
+                                          (λs. Ret' s)
+                                          (λt. Tau' (INR t))
+                                          (λe g. Vis' e (INR ∘ g))
+  ∧ ibind_cb k (INL (Tau t)) = Tau' (INL t)
+  ∧ ibind_cb k (INL (Vis e g)) = Vis' e (INL ∘ g)
+  ∧ ibind_cb k (INR (Ret r')) = Ret' r'
+  ∧ ibind_cb k (INR (Tau t')) = Tau' (INR t')
+  ∧ ibind_cb k (INR (Vis e' g')) = Vis' e' (INR ∘ g')
+End
+
+Theorem itree_bind_alt1:
+  itree_bind t k = itree_unfold (ibind_cb k) (INL t)
+Proof
+  rw[itree_bind_def] >>
+  AP_THM_TAC >>
+  AP_TERM_TAC >>
+  rw[FUN_EQ_THM] >>
+  rw[DefnBase.one_line_ify NONE ibind_cb_def]
+QED
+
+(* manual unrolling hack to get the cb simp to fire *)
+Theorem itree_bind_alt:
+  itree_bind t k = case ibind_cb k (INL t) of
+                     Ret' r => Ret r
+                   | Tau' s => Tau (itree_unfold (ibind_cb k) s)
+                   | Vis' e g => Vis e (itree_unfold (ibind_cb k) ∘ g)
+Proof
+  CONV_TAC $ LHS_CONV $ ONCE_REWRITE_CONV[itree_bind_alt1] >>
+  rw[Once itree_unfold]
+QED
+
+(* won't loop because (ibind_cb (INR Ret)) only produces Ret *)
+Theorem itree_unfold_ibind_INR_Ret:
+  itree_unfold (ibind_cb k) (INR (Ret r)) = Ret r
+Proof
+  rw[Once itree_unfold]
+QED
+
+(* itree iter *)
+
+Definition iiter_cb_def[simp]:
+    iiter_cb body (Ret (INL cont)) = Tau' (body cont)
+  ∧ iiter_cb body (Ret (INR r))    = Ret' r
+  ∧ iiter_cb body (Tau t) = Tau' t
+  ∧ iiter_cb body (Vis e g) = Vis' e g
+End
+
+Theorem itree_iter_alt1:
+  itree_iter body seed = itree_unfold (iiter_cb body) (body seed)
+Proof
+  rw[itree_iter_def] >>
+  AP_THM_TAC >>
+  AP_TERM_TAC >>
+  rw[FUN_EQ_THM] >>
+  rw[DefnBase.one_line_ify NONE iiter_cb_def]
+QED
+
+Theorem itree_iter_alt:
+  itree_iter body seed = case iiter_cb body (body seed) of
+                           Ret' r => Ret r
+                         | Tau' s => Tau (itree_unfold (iiter_cb body) s)
+                         | Vis' e g => Vis e (itree_unfold (iiter_cb body) ∘ g)
+Proof
+  CONV_TAC $ LHS_CONV $ ONCE_REWRITE_CONV[itree_iter_alt1] >>
+  rw[Once itree_unfold]
+QED
+
+Theorem itree_unfold_iiter_Ret_INL:
+  itree_unfold (iiter_cb k) (Ret (INL r)) = Tau (itree_unfold (iiter_cb k) (k r))
+Proof
+  rw[Once itree_unfold]
+QED
+
+Theorem itree_unfold_iiter_Ret_INR:
+  itree_unfold (iiter_cb k) (Ret (INR r)) = Ret r
+Proof
+  rw[Once itree_unfold]
+QED
+
+(* massage Ret type from (η x state) -> η *)
+(* convert Vis (sem_vis_event x (FFI_result -> itree)) ((prog x state) -> %itree)
+-> Vis sem_vis_event (FFI_result -> itree) *)
+
+Definition massage_def[simp]:
+    massage (INL (Ret (res, s))) = Ret' res
+  ∧ massage (INR (Ret (res',s'))) = Ret' res'
+  ∧ massage (INL (Tau t)) = Tau' (INL t)
+  ∧ massage (INR (Tau t')) = Tau' (INR t')
+  ∧ massage (INL (Vis (e,k) g)) = Vis' e (λr. INR (k r))
+  ∧ massage (INR (Vis e'    g')) = Vis' e' (INR ∘ g')
+End
+
+Theorem itree_evaluate_alt:
+  itree_evaluate p s = itree_unfold massage (INL (itree_mrec h_prog (p,s)))
+Proof
+  rw[itree_evaluate_def] >>
+  AP_THM_TAC >> (* same fn => same on same arg, backwards *)
+  AP_TERM_TAC >>
+  rw[FUN_EQ_THM] >>
+  rw[DefnBase.one_line_ify NONE massage_def]
+QED
+
+Definition mrec_cb_def[simp]:
+  mrec_cb rh (Ret r) = Ret (INR r) ∧
+  mrec_cb rh (Tau t) = Ret (INL t) ∧
+  mrec_cb rh (Vis (INL state_res) k) = Ret (INL (⋆ (rh state_res) k)) ∧
+  mrec_cb rh (Vis (INR ffi_res) k) = Vis ffi_res (λx. Ret (INL (k x)))
+End
+
+Theorem itree_mrec_alt:
+  itree_mrec rh seed = itree_iter (mrec_cb rh) (rh seed)
+Proof
+  rw[itree_mrec_def] >>
+  AP_THM_TAC >>
+  AP_TERM_TAC >>
+  rw[FUN_EQ_THM] >>
+  rw[DefnBase.one_line_ify NONE mrec_cb_def]
+QED
+
+(* Theorem itree_mrec_dec: *)
+(*   itree_mrec ((Dec x exp prog),s) = *)
+(*   case eval s exp of *)
+(*     NONE => Ret(SOME Error) *)
+(*   | SOME value => *)
+(*       (Tau (itree_mrec prog (s with locals := s.locals |+ (x,value)))) *)
+(* Proof *)
+(*   rw[itree_semantics_def, itree_evaluate_alt] >> *)
+(*   rw[Once itree_mrec_def, h_prog_def, h_prog_rule_dec_def] >> *)
+(*   BasicProvers.PURE_TOP_CASE_TAC >> *)
+(*   gvs[itree_iter_def] >- *)
+(*    (rw[Once itree_unfold] >> *)
+(*     rw[Once itree_unfold]) >> *)
+
+(*   rw[Once itree_mrec_def] >> *)
+(*   rw[itree_iter_def] >> *)
+
+(*   unfold_inner >> rw[] >> *)
+(*   CONV_TAC $ LHS_CONV $ SIMP_CONV std_ss[Once itree_unfold, massage_def] >> rw[] >> *)
+(*   (* internal itree type doesn't match *) *)
+(* QED *)
+
+(* RAND_CONV : f x (unfold) -> x *)
+
+Definition mrec_test_def:
+  mrec_test (s:('a,'ffi) panSem$state)
+  = itree_evaluate (Seq Skip (Return (Const 42w))) s
+End
+
+Theorem itree_mrec_test:
+  mrec_test s = Tau (Tau (Ret (SOME (Return (ValWord 42w)))))
+Proof
+  rw[mrec_test_def, itree_evaluate_alt] >>
+  rw[itree_mrec_alt, h_prog_def] >>
+  rw[h_prog_rule_seq_def] >>
+  rw[itree_iter_alt] >>
+  rw[h_prog_def] >>
+  rw[itree_bind_alt] >>
+  rw[itree_trigger_def] >>
+  (* return *)
+  rw[h_prog_def,h_prog_rule_return_def,size_of_shape_def,shape_of_def,eval_def] >>
+  rw[itree_bind_alt, itree_unfold_ibind_INR_Ret] >>
+  rw[itree_unfold_iiter_Ret_INL] >>
+  rw[itree_unfold_iiter_Ret_INR] >>
+  rw[Once itree_unfold, massage_def] >>
+  rw[Once itree_unfold, massage_def] >>
+  rw[Once itree_unfold, massage_def]
+QED
+
 (* pancake programs *)
 
 local
